language_formal/spark2014_semantics/spark2014_core_subset(non-nested)/checks_generator.v
@@ -1,5 +1,5 @@
 Require Export language_flagged.
-
+Require Export symboltable.
 
 (* ***************************************************************
    generate and insert check flags into AST nodes according to the 
@@ -7,81 +7,146 @@ Require Export language_flagged.
    *************************************************************** *)
 
 (** * Compile To Flagged Program *)
+(** check flags for an expression not only depends on its operators, 
+    but also depends on its context where it appears, e.g. if it's 
+    used as an index, then Do_Range_Check should be set for it;
+    in the following formalization, check_flags are the check flags
+    that are enforced by the context of the expression;
+*)
 
-Inductive compile2_flagged_exp: expression -> expression_x -> Prop :=
-    | C2_Flagged_Literal: forall ast_num l checkflags,
-        gen_exp_check_flags (E_Literal ast_num l) checkflags ->
-        compile2_flagged_exp (E_Literal ast_num l) (E_Literal_X ast_num l checkflags) 
-    | C2_Flagged_Name: forall ast_num n checkflags n_flagged,
-        gen_exp_check_flags (E_Name ast_num n) checkflags ->
-        compile2_flagged_name n n_flagged ->
-        compile2_flagged_exp (E_Name ast_num n) (E_Name_X ast_num n_flagged checkflags) 
-    | C2_Flagged_Binary_Operation: forall ast_num op e1 e2 checkflags e1_flagged e2_flagged,
-        gen_exp_check_flags (E_Binary_Operation ast_num op e1 e2) checkflags ->
-        compile2_flagged_exp e1 e1_flagged ->
-        compile2_flagged_exp e2 e2_flagged ->
-        compile2_flagged_exp (E_Binary_Operation ast_num op e1 e2)
+Inductive compile2_flagged_exp: check_flags -> expression -> expression_x -> Prop :=
+    | C2_Flagged_Literal: forall checkflags ast_num l,
+        compile2_flagged_exp checkflags 
+                             (E_Literal ast_num l) 
+                             (E_Literal_X ast_num l checkflags)
+    | C2_Flagged_Name: forall checkflags n n_flagged ast_num,
+        compile2_flagged_name checkflags n n_flagged -> (* checkflags is passed into name expression *)
+        compile2_flagged_exp checkflags 
+                             (E_Name ast_num n) 
+                             (E_Name_X ast_num n_flagged nil)
+    | C2_Flagged_Binary_Operation_O: forall op e1 e1_flagged e2 e2_flagged checkflags ast_num,
+        op = Plus \/ op = Minus \/ op = Multiply ->
+        compile2_flagged_exp nil e1 e1_flagged ->
+        compile2_flagged_exp nil e2 e2_flagged ->
+        compile2_flagged_exp checkflags
+                             (E_Binary_Operation ast_num op e1 e2)
+                             (E_Binary_Operation_X ast_num op e1_flagged e2_flagged (Do_Overflow_Check :: checkflags))
+    | C2_Flagged_Binary_Operation_OD: forall op e1 e1_flagged e2 e2_flagged checkflags ast_num,
+        op = Divide ->
+        compile2_flagged_exp nil e1 e1_flagged ->
+        compile2_flagged_exp nil e2 e2_flagged ->
+        compile2_flagged_exp checkflags
+                             (E_Binary_Operation ast_num op e1 e2)
+                             (E_Binary_Operation_X ast_num op e1_flagged e2_flagged (Do_Division_Check :: Do_Overflow_Check :: checkflags))
+    | C2_Flagged_Binary_Operation_Others: forall op e1 e1_flagged e2 e2_flagged checkflags ast_num,
+        op <> Plus ->
+        op <> Minus ->
+        op <> Multiply ->
+        op <> Divide ->
+        compile2_flagged_exp nil e1 e1_flagged ->
+        compile2_flagged_exp nil e2 e2_flagged ->
+        compile2_flagged_exp checkflags
+                             (E_Binary_Operation ast_num op e1 e2)
                              (E_Binary_Operation_X ast_num op e1_flagged e2_flagged checkflags)
-    | C2_Flagged_Unary_Operation: forall ast_num op e checkflags e_flagged,
-        gen_exp_check_flags (E_Unary_Operation ast_num op e) checkflags ->
-        compile2_flagged_exp e e_flagged ->
-        compile2_flagged_exp (E_Unary_Operation ast_num op e) 
+    | C2_Flagged_Unary_Operation_O: forall op e e_flagged checkflags ast_num,
+        op = Unary_Minus ->
+        compile2_flagged_exp nil e e_flagged ->
+        compile2_flagged_exp checkflags
+                             (E_Unary_Operation ast_num op e) 
+                             (E_Unary_Operation_X ast_num op e_flagged (Do_Overflow_Check :: checkflags))
+    | C2_Flagged_Unary_Operation_Others: forall op e e_flagged checkflags ast_num,
+        op <> Unary_Minus ->
+        compile2_flagged_exp nil e e_flagged ->
+        compile2_flagged_exp checkflags
+                             (E_Unary_Operation ast_num op e) 
                              (E_Unary_Operation_X ast_num op e_flagged checkflags)
-        
-with compile2_flagged_name: name -> name_x -> Prop :=
-    | C2_Flagged_Identifier: forall ast_num x checkflags,
-        gen_name_check_flags (E_Identifier ast_num x) checkflags ->
-        compile2_flagged_name (E_Identifier ast_num x) (E_Identifier_X ast_num x checkflags) 
-    | C2_Flagged_Indexed_Component: forall ast_num x_ast_num x e checkflags e_flagged,
-        gen_name_check_flags (E_Indexed_Component ast_num x_ast_num x e) checkflags ->
-        compile2_flagged_exp e e_flagged ->
-        compile2_flagged_name (E_Indexed_Component ast_num x_ast_num x e) 
+
+with compile2_flagged_name: check_flags -> name -> name_x -> Prop :=
+    | C2_Flagged_Identifier: forall checkflags ast_num x,
+        compile2_flagged_name checkflags 
+                              (E_Identifier ast_num x) 
+                              (E_Identifier_X ast_num x checkflags) 
+    | C2_Flagged_Indexed_Component: forall e e_flagged checkflags ast_num x_ast_num x,
+        compile2_flagged_exp (Do_Range_Check :: nil) e e_flagged ->
+        compile2_flagged_name checkflags
+                              (E_Indexed_Component ast_num x_ast_num x e) 
                               (E_Indexed_Component_X ast_num x_ast_num x e_flagged checkflags) 
-    | C2_Flagged_Selected_Component: forall ast_num x_ast_num x f checkflags,
-        gen_name_check_flags (E_Selected_Component ast_num x_ast_num x f) checkflags ->
-        compile2_flagged_name (E_Selected_Component ast_num x_ast_num x f) 
+    | C2_Flagged_Selected_Component: forall checkflags ast_num x_ast_num x f,
+        compile2_flagged_name checkflags 
+                              (E_Selected_Component ast_num x_ast_num x f) 
                               (E_Selected_Component_X ast_num x_ast_num x f checkflags).
 
-Inductive compile2_flagged_exps: list expression -> list expression_x -> Prop :=
-    | C2_Flagged_Exps_Null:
-        compile2_flagged_exps nil nil 
-    | C2_Flagged_Exps_List: forall e e_flagged le le_flagged,
-        compile2_flagged_exp  e  e_flagged ->
-        compile2_flagged_exps le le_flagged ->
-        compile2_flagged_exps (e :: le) (e_flagged :: le_flagged).
+Inductive compile2_flagged_args: list parameter_specification -> list expression -> list expression_x -> Prop :=
+    | C2_Flagged_Args_Null:
+        compile2_flagged_args nil nil nil
+    | C2_Flagged_Args: forall param arg arg_flagged lparam larg larg_flagged,
+        is_range_constrainted_type (param.(parameter_subtype_mark)) = false ->
+        compile2_flagged_exp nil arg arg_flagged ->
+        compile2_flagged_args lparam larg larg_flagged -> 
+        compile2_flagged_args (param :: lparam) (arg :: larg) (arg_flagged :: larg_flagged)
+    | C2_Flagged_Args_R: forall param arg arg_flagged lparam larg larg_flagged,
+        is_range_constrainted_type (param.(parameter_subtype_mark)) = true ->
+        compile2_flagged_exp (Do_Range_Check :: nil) arg arg_flagged ->
+        compile2_flagged_args lparam larg larg_flagged -> 
+        compile2_flagged_args (param :: lparam) (arg :: larg) (arg_flagged :: larg_flagged).
 
-
-Inductive compile2_flagged_stmt: statement -> statement_x -> Prop := 
-    | C2_Flagged_Null:
-        compile2_flagged_stmt S_Null S_Null_X 
-    | C2_Flagged_Assignment: forall x x_flagged e e_flagged ast_num,
-        compile2_flagged_name x x_flagged ->
-        compile2_flagged_exp  e e_flagged -> 
-        compile2_flagged_stmt (S_Assignment   ast_num x e) 
-                              (S_Assignment_X ast_num x_flagged e_flagged) 
-    | C2_Flagged_If: forall e e_flagged c1 c1_flagged c2 c2_flagged ast_num,
-        compile2_flagged_exp  e  e_flagged ->
-        compile2_flagged_stmt c1 c1_flagged ->
-        compile2_flagged_stmt c2 c2_flagged ->
-        compile2_flagged_stmt (S_If   ast_num e c1 c2) 
+Inductive compile2_flagged_stmt: symboltable -> statement -> statement_x -> Prop := 
+    | C2_Flagged_Null: forall st,
+        compile2_flagged_stmt st S_Null S_Null_X
+    | C2_Flagged_Assignment: forall x st t x_flagged e e_flagged ast_num,
+        fetch_exp_type (name_astnum x) st = Some t ->
+        is_range_constrainted_type t = false ->        
+        compile2_flagged_name nil x x_flagged ->
+        compile2_flagged_exp  nil e e_flagged ->
+        compile2_flagged_stmt st
+                              (S_Assignment   ast_num x e) 
+                              (S_Assignment_X ast_num x_flagged e_flagged)
+    | C2_Flagged_Assignment_R: forall x st t x_flagged e e_flagged ast_num,
+        fetch_exp_type (name_astnum x) st = Some t ->
+        is_range_constrainted_type t = true ->
+        compile2_flagged_name nil x x_flagged ->
+        compile2_flagged_exp  (Do_Range_Check :: nil) e e_flagged ->
+        compile2_flagged_stmt st
+                              (S_Assignment   ast_num x e)
+                              (S_Assignment_X ast_num x_flagged e_flagged)
+    | C2_Flagged_If: forall e e_flagged c1 c1_flagged c2 c2_flagged st ast_num,
+        compile2_flagged_exp  nil e e_flagged ->
+        compile2_flagged_stmt st c1 c1_flagged ->
+        compile2_flagged_stmt st c2 c2_flagged ->
+        compile2_flagged_stmt st
+                              (S_If   ast_num e c1 c2) 
                               (S_If_X ast_num e_flagged c1_flagged c2_flagged)
-    | C2_Flagged_While: forall e e_flagged c c_flagged ast_num,
-        compile2_flagged_exp  e e_flagged ->
-        compile2_flagged_stmt c c_flagged ->
-        compile2_flagged_stmt (S_While_Loop   ast_num e c) 
+    | C2_Flagged_While: forall e e_flagged c c_flagged st ast_num,
+        compile2_flagged_exp  nil e e_flagged ->
+        compile2_flagged_stmt st c c_flagged ->
+        compile2_flagged_stmt st 
+                              (S_While_Loop   ast_num e c) 
                               (S_While_Loop_X ast_num e_flagged c_flagged)
-    | C2_Flagged_Procedure_Call: forall args args_flagged ast_num p_ast_num p,
-        compile2_flagged_exps args args_flagged ->
-        compile2_flagged_stmt (S_Procedure_Call   ast_num p_ast_num p args) 
+    | C2_Flagged_Procedure_Call: forall p st n pb params args args_flagged ast_num p_ast_num,
+        fetch_proc p st = Some (n, pb) ->
+        procedure_parameter_profile pb = params ->
+        compile2_flagged_args params args args_flagged ->
+        compile2_flagged_stmt st
+                              (S_Procedure_Call   ast_num p_ast_num p args) 
                               (S_Procedure_Call_X ast_num p_ast_num p args_flagged)
-    | C2_Flagged_Sequence: forall c1 c1_flagged c2 c2_flagged ast_num,
-        compile2_flagged_stmt c1 c1_flagged ->
-        compile2_flagged_stmt c2 c2_flagged ->
-        compile2_flagged_stmt (S_Sequence ast_num   c1 c2)
+    | C2_Flagged_Sequence: forall st c1 c1_flagged c2 c2_flagged ast_num,
+        compile2_flagged_stmt st c1 c1_flagged ->
+        compile2_flagged_stmt st c2 c2_flagged ->
+        compile2_flagged_stmt st
+                              (S_Sequence ast_num   c1 c2)
                               (S_Sequence_X ast_num c1_flagged c2_flagged).
 
 
 Inductive compile2_flagged_type_declaration: type_declaration -> type_declaration_x -> Prop :=
+    | C2_Flagged_Subtype_Decl: forall ast_num tn t l u,
+        compile2_flagged_type_declaration (Subtype_Declaration   ast_num tn t l u)
+                                          (Subtype_Declaration_X ast_num tn t l u)
+    | C2_Flagged_Derived_Type_Decl: forall ast_num tn t l u,
+        compile2_flagged_type_declaration (Derived_Type_Declaration   ast_num tn t l u)
+                                          (Derived_Type_Declaration_X ast_num tn t l u)
+    | C2_Flagged_Integer_Type_Decl: forall ast_num tn l u,
+        compile2_flagged_type_declaration (Integer_Type_Declaration   ast_num tn l u)
+                                          (Integer_Type_Declaration_X ast_num tn l u)
     | C2_Flagged_Array_Type_Decl: forall ast_num tn t l u,
         compile2_flagged_type_declaration (Array_Type_Declaration   ast_num tn t l u)
                                           (Array_Type_Declaration_X ast_num tn t l u)
@@ -89,13 +154,18 @@ Inductive compile2_flagged_type_declaration: type_declaration -> type_declaratio
         compile2_flagged_type_declaration (Record_Type_Declaration   ast_num tn fs) 
                                           (Record_Type_Declaration_X ast_num tn fs).
 
-
 Inductive compile2_flagged_object_declaration: object_declaration -> object_declaration_x -> Prop :=
     | C2_Flagged_Object_Declaration_NoneInit: forall ast_num x t,
         compile2_flagged_object_declaration (mkobject_declaration   ast_num x t None) 
                                             (mkobject_declaration_x ast_num x t None) 
-    | C2_Flagged_Object_Declaration: forall e e_flagged ast_num x t,
-        compile2_flagged_exp e e_flagged ->
+    | C2_Flagged_Object_Declaration: forall t e e_flagged ast_num x,
+        is_range_constrainted_type t = false ->
+        compile2_flagged_exp nil e e_flagged ->
+        compile2_flagged_object_declaration (mkobject_declaration   ast_num x t (Some e)) 
+                                            (mkobject_declaration_x ast_num x t (Some e_flagged))
+    | C2_Flagged_Object_Declaration_R: forall t e e_flagged ast_num x,
+        is_range_constrainted_type t = true ->
+        compile2_flagged_exp (Do_Range_Check :: nil) e e_flagged ->
         compile2_flagged_object_declaration (mkobject_declaration   ast_num x t (Some e)) 
                                             (mkobject_declaration_x ast_num x t (Some e_flagged)).
 
@@ -122,50 +192,40 @@ Inductive compile2_flagged_parameter_specifications: list parameter_specificatio
         compile2_flagged_parameter_specifications (param :: lparam) (param_flagged :: lparam_flagged).
 
 
-Inductive compile2_flagged_aspect_specification: aspect_specification -> aspect_specification_x -> Prop :=
-    | C2_Flagged_Aspect_Spec: forall e e_flagged ast_num mk,
-        compile2_flagged_exp e e_flagged ->
-        compile2_flagged_aspect_specification (mkaspect_specification   ast_num mk e) 
-                                              (mkaspect_specification_x ast_num mk e_flagged).
-
-Inductive compile2_flagged_aspect_specifications: list aspect_specification -> list aspect_specification_x -> Prop :=
-    | C2_Flagged_Aspect_Specs_Null: 
-        compile2_flagged_aspect_specifications nil nil 
-    | C2_Flagged_Aspect_Specs_List: forall aspect aspect_flagged laspect laspect_flagged,
-        compile2_flagged_aspect_specification  aspect  aspect_flagged ->
-        compile2_flagged_aspect_specifications laspect laspect_flagged ->
-        compile2_flagged_aspect_specifications (aspect :: laspect) (aspect_flagged :: laspect_flagged).
-
-
-Inductive compile2_flagged_declaration: declaration -> declaration_x -> Prop :=
-    | C2_Flagged_D_Null_Declaration: 
-        compile2_flagged_declaration D_Null_Declaration D_Null_Declaration_X
-    | C2_Flagged_D_Type_Declaration: forall t t_flagged ast_num,
+Inductive compile2_flagged_declaration: symboltable -> declaration -> declaration_x -> Prop :=
+    | C2_Flagged_D_Null_Declaration: forall st,
+        compile2_flagged_declaration st D_Null_Declaration D_Null_Declaration_X
+    | C2_Flagged_D_Type_Declaration: forall t t_flagged st ast_num,
         compile2_flagged_type_declaration t t_flagged ->
-        compile2_flagged_declaration (D_Type_Declaration   ast_num t) 
+        compile2_flagged_declaration st
+                                     (D_Type_Declaration   ast_num t) 
                                      (D_Type_Declaration_X ast_num t_flagged)
-    | C2_Flagged_D_Object_Declaration: forall o o_flagged ast_num,
+    | C2_Flagged_D_Object_Declaration: forall o o_flagged st ast_num,
         compile2_flagged_object_declaration o o_flagged ->
-        compile2_flagged_declaration (D_Object_Declaration   ast_num o)
+        compile2_flagged_declaration st 
+                                     (D_Object_Declaration   ast_num o)
                                      (D_Object_Declaration_X ast_num o_flagged) 
-    | C2_Flagged_D_Procedure_Declaration: forall p p_flagged ast_num,
-        compile2_flagged_procedure_body p p_flagged ->
-        compile2_flagged_declaration (D_Procedure_Body   ast_num p)
+    | C2_Flagged_D_Procedure_Declaration: forall st p p_flagged ast_num,
+        compile2_flagged_procedure_body st p p_flagged ->
+        compile2_flagged_declaration st 
+                                     (D_Procedure_Body   ast_num p)
                                      (D_Procedure_Body_X ast_num p_flagged) 
-    | C2_Flagged_D_Seq_Declaration: forall d1 d1_flagged d2 d2_flagged ast_num,
-        compile2_flagged_declaration d1 d1_flagged ->
-        compile2_flagged_declaration d2 d2_flagged ->
-        compile2_flagged_declaration (D_Seq_Declaration ast_num d1 d2) (D_Seq_Declaration_X ast_num d1_flagged d2_flagged)
+    | C2_Flagged_D_Seq_Declaration: forall st d1 d1_flagged d2 d2_flagged ast_num,
+        compile2_flagged_declaration st d1 d1_flagged ->
+        compile2_flagged_declaration st d2 d2_flagged ->
+        compile2_flagged_declaration st 
+                                     (D_Seq_Declaration   ast_num d1 d2) 
+                                     (D_Seq_Declaration_X ast_num d1_flagged d2_flagged)
 
-with compile2_flagged_procedure_body: procedure_body -> procedure_body_x -> Prop :=
-       | C2_Flagged_Procedure_Declaration: forall aspects aspects_flagged params params_flagged 
-                                                  decls decls_flagged stmt stmt_flagged ast_num p,
-           compile2_flagged_aspect_specifications aspects aspects_flagged ->
+with compile2_flagged_procedure_body: symboltable -> procedure_body -> procedure_body_x -> Prop :=
+       | C2_Flagged_Procedure_Declaration: forall params params_flagged st decls decls_flagged
+                                                  stmt stmt_flagged ast_num p,
            compile2_flagged_parameter_specifications params params_flagged ->
-           compile2_flagged_declaration decls decls_flagged ->
-           compile2_flagged_stmt stmt stmt_flagged ->
-           compile2_flagged_procedure_body (mkprocedure_body   ast_num p params aspects decls stmt)
-                                                  (mkprocedure_body_x ast_num p params_flagged aspects_flagged decls_flagged stmt_flagged).
+           compile2_flagged_declaration st decls decls_flagged ->
+           compile2_flagged_stmt st stmt stmt_flagged ->
+           compile2_flagged_procedure_body st 
+                                           (mkprocedure_body   ast_num p params decls stmt)
+                                           (mkprocedure_body_x ast_num p params_flagged decls_flagged stmt_flagged).
 
 
 (* ***************************************************************
@@ -174,89 +234,138 @@ with compile2_flagged_procedure_body: procedure_body -> procedure_body_x -> Prop
 
 (** * Translator Function To Insert Checks *)
 
-Function compile2_flagged_exp_f (e: expression): expression_x :=
+Function compile2_flagged_exp_f (checkflags: check_flags) (e: expression): expression_x :=
   match e with
   | E_Literal ast_num l => 
-      let checkflags := gen_exp_check_flags_f (E_Literal ast_num l) in
-        (E_Literal_X ast_num l checkflags)
+        E_Literal_X ast_num l checkflags
   | E_Name ast_num n => 
-      let checkflags := gen_exp_check_flags_f (E_Name ast_num n) in
-      let n_flagged := compile2_flagged_name_f n in
-        (E_Name_X ast_num n_flagged checkflags)
+      let n_flagged := compile2_flagged_name_f checkflags n in
+        E_Name_X ast_num n_flagged nil
   | E_Binary_Operation ast_num op e1 e2 =>
-      let checkflags := gen_exp_check_flags_f (E_Binary_Operation ast_num op e1 e2) in
-      let e1_flagged := compile2_flagged_exp_f e1 in
-      let e2_flagged := compile2_flagged_exp_f e2 in
-        (E_Binary_Operation_X ast_num op e1_flagged e2_flagged checkflags)
+      let e1_flagged := compile2_flagged_exp_f nil e1 in
+      let e2_flagged := compile2_flagged_exp_f nil e2 in
+        match op with
+        | Plus     => E_Binary_Operation_X ast_num op e1_flagged e2_flagged (Do_Overflow_Check :: checkflags)
+        | Minus    => E_Binary_Operation_X ast_num op e1_flagged e2_flagged (Do_Overflow_Check :: checkflags)
+        | Multiply => E_Binary_Operation_X ast_num op e1_flagged e2_flagged (Do_Overflow_Check :: checkflags)
+        | Divide   => E_Binary_Operation_X ast_num op e1_flagged e2_flagged (Do_Division_Check :: Do_Overflow_Check :: checkflags)
+        | _        => E_Binary_Operation_X ast_num op e1_flagged e2_flagged checkflags
+        end
   | E_Unary_Operation ast_num op e => 
-      let checkflags := gen_exp_check_flags_f (E_Unary_Operation ast_num op e) in
-      let e_flagged := compile2_flagged_exp_f e in
-        (E_Unary_Operation_X ast_num op e_flagged checkflags)
+      let e_flagged := compile2_flagged_exp_f nil e in
+        match op with
+        | Unary_Minus => E_Unary_Operation_X ast_num op e_flagged (Do_Overflow_Check :: checkflags)
+        | _           => E_Unary_Operation_X ast_num op e_flagged checkflags
+        end
   end
 
-with compile2_flagged_name_f (n: name): name_x :=
+with compile2_flagged_name_f (checkflags: check_flags) (n: name): name_x :=
   match n with
   | E_Identifier ast_num x =>
-      let checkflags := gen_name_check_flags_f (E_Identifier ast_num x) in
-        (E_Identifier_X ast_num x checkflags)
+        E_Identifier_X ast_num x checkflags
   | E_Indexed_Component ast_num x_ast_num x e =>
-      let checkflags := gen_name_check_flags_f (E_Indexed_Component ast_num x_ast_num x e) in
-      let e_flagged := compile2_flagged_exp_f e in
-        (E_Indexed_Component_X ast_num x_ast_num x e_flagged checkflags)
+      let e_flagged := compile2_flagged_exp_f (Do_Range_Check :: nil) e in
+        E_Indexed_Component_X ast_num x_ast_num x e_flagged checkflags
   | E_Selected_Component ast_num x_ast_num x f =>
-      let checkflags := gen_name_check_flags_f (E_Selected_Component ast_num x_ast_num x f) in
-        (E_Selected_Component_X ast_num x_ast_num x f checkflags)
+        E_Selected_Component_X ast_num x_ast_num x f checkflags
   end.
 
-Function compile2_flagged_exps_f (le: list expression): list expression_x :=
-  match le with
-  | nil => nil
-  | e :: le' => 
-      let e_flagged := compile2_flagged_exp_f e in
-      let le_flagged := compile2_flagged_exps_f le' in
-        (e_flagged :: le_flagged)
+Function compile2_flagged_args_f (params: list parameter_specification) (args: list expression): option (list expression_x) :=
+  match params, args with
+  | nil, nil => Some nil
+  | param :: params', arg :: args' =>
+      if is_range_constrainted_type (param.(parameter_subtype_mark)) then
+        let arg_flagged := compile2_flagged_exp_f (Do_Range_Check :: nil) arg in
+        match compile2_flagged_args_f params' args' with
+        | Some args_flagged => Some (arg_flagged :: args_flagged)
+        | None              => None
+        end
+      else
+        let arg_flagged := compile2_flagged_exp_f nil arg in
+        match compile2_flagged_args_f params' args' with
+        | Some args_flagged => Some (arg_flagged :: args_flagged)
+        | None              => None
+        end
+  | _, _ => None
   end.
 
-Function compile2_flagged_stmt_f (c: statement): statement_x :=
+Function compile2_flagged_stmt_f (st: symboltable) (c: statement): option statement_x :=
   match c with
-  | S_Null => S_Null_X
+  | S_Null => Some S_Null_X
   | S_Assignment ast_num x e =>
-      let x_flagged := compile2_flagged_name_f x in
-      let e_flagged := compile2_flagged_exp_f  e in
-        (S_Assignment_X ast_num x_flagged e_flagged)
+      match fetch_exp_type (name_astnum x) st with
+      | Some t =>
+          if is_range_constrainted_type t then
+            let x_flagged := compile2_flagged_name_f nil x in
+            let e_flagged := compile2_flagged_exp_f  (Do_Range_Check :: nil) e in
+              Some (S_Assignment_X ast_num x_flagged e_flagged) 
+          else
+            let x_flagged := compile2_flagged_name_f nil x in
+            let e_flagged := compile2_flagged_exp_f  nil e in
+              Some (S_Assignment_X ast_num x_flagged e_flagged)
+      | None   => None
+      end
   | S_If ast_num e c1 c2 =>
-      let e_flagged := compile2_flagged_exp_f e in
-      let c1_flagged := compile2_flagged_stmt_f c1 in
-      let c2_flagged := compile2_flagged_stmt_f c2 in
-        (S_If_X ast_num e_flagged c1_flagged c2_flagged)
+      let e_flagged := compile2_flagged_exp_f nil e in
+        match compile2_flagged_stmt_f st c1 with
+        | Some c1_flagged =>
+            match compile2_flagged_stmt_f st c2 with
+            | Some c2_flagged => Some (S_If_X ast_num e_flagged c1_flagged c2_flagged)
+            | None            => None
+            end
+        | None            => None
+        end
   | S_While_Loop ast_num e c =>
-      let e_flagged := compile2_flagged_exp_f e in
-      let c_flagged := compile2_flagged_stmt_f c in
-        (S_While_Loop_X ast_num e_flagged c_flagged)
+      let e_flagged := compile2_flagged_exp_f nil e in
+        match compile2_flagged_stmt_f st c with
+        | Some c_flagged => Some (S_While_Loop_X ast_num e_flagged c_flagged)
+        | None           => None
+        end
   | S_Procedure_Call ast_num p_ast_num p args =>
-      let args_flagged := compile2_flagged_exps_f args in
-        (S_Procedure_Call_X ast_num p_ast_num p args_flagged)
+      match fetch_proc p st with
+      | Some (n, pb) => 
+          match compile2_flagged_args_f (procedure_parameter_profile pb) args with
+          | Some args_flagged => Some (S_Procedure_Call_X ast_num p_ast_num p args_flagged)
+          | None              => None
+          end
+      | None         => None
+      end
   | S_Sequence ast_num c1 c2 =>
-      let c1_flagged := compile2_flagged_stmt_f c1 in
-      let c2_flagged := compile2_flagged_stmt_f c2 in
-        (S_Sequence_X ast_num c1_flagged c2_flagged)
+      match compile2_flagged_stmt_f st c1 with
+      | Some c1_flagged =>
+          match compile2_flagged_stmt_f st c2 with
+          | Some c2_flagged => Some (S_Sequence_X ast_num c1_flagged c2_flagged)
+          | None            => None
+          end
+      | None            => None
+      end
   end.
 
 Function compile2_flagged_type_declaration_f (t: type_declaration): type_declaration_x :=
   match t with
+  | Subtype_Declaration ast_num tn t l u =>
+      Subtype_Declaration_X ast_num tn t l u
+  | Derived_Type_Declaration ast_num tn t l u =>
+      Derived_Type_Declaration_X ast_num tn t l u
+  | Integer_Type_Declaration ast_num tn l u =>
+      Integer_Type_Declaration_X ast_num tn l u
   | Array_Type_Declaration ast_num tn t l u => 
-      (Array_Type_Declaration_X ast_num tn t l u)
+      Array_Type_Declaration_X ast_num tn t l u
   | Record_Type_Declaration ast_num tn fs =>
-      (Record_Type_Declaration_X ast_num tn fs)
+      Record_Type_Declaration_X ast_num tn fs
   end.
 
 Function compile2_flagged_object_declaration_f (o: object_declaration): object_declaration_x :=
   match o with
   | mkobject_declaration ast_num x t None =>
-      (mkobject_declaration_x ast_num x t None)
+        mkobject_declaration_x ast_num x t None
   | mkobject_declaration ast_num x t (Some e) => 
-      let e_flagged := compile2_flagged_exp_f e in
-        (mkobject_declaration_x ast_num x t (Some e_flagged))
+      if is_range_constrainted_type t then
+        let e_flagged := compile2_flagged_exp_f (Do_Range_Check :: nil) e in
+          mkobject_declaration_x ast_num x t (Some e_flagged) 
+      else
+        let e_flagged := compile2_flagged_exp_f nil e in
+          mkobject_declaration_x ast_num x t (Some e_flagged)
   end.
 
 Function compile2_flagged_object_declarations_f (lo: list object_declaration): list object_declaration_x :=
@@ -265,13 +374,13 @@ Function compile2_flagged_object_declarations_f (lo: list object_declaration): l
   | o :: lo' => 
       let o_flagged := compile2_flagged_object_declaration_f o in
       let lo_flagged := compile2_flagged_object_declarations_f lo' in
-        (o_flagged :: lo_flagged)
+        o_flagged :: lo_flagged
   end.
 
 Function compile2_flagged_parameter_specification_f (param: parameter_specification): parameter_specification_x :=
   match param with
-  | mkparameter_specification   ast_num x t m =>
-      (mkparameter_specification_x ast_num x t m)
+  | mkparameter_specification ast_num x t m =>
+      mkparameter_specification_x ast_num x t m
   end.
 
 Function compile2_flagged_parameter_specifications_f (lparam: list parameter_specification): list parameter_specification_x :=
@@ -280,81 +389,48 @@ Function compile2_flagged_parameter_specifications_f (lparam: list parameter_spe
   | param :: lparam' =>
       let param_flagged := compile2_flagged_parameter_specification_f param in
       let lparam_flagged := compile2_flagged_parameter_specifications_f lparam' in
-        (param_flagged :: lparam_flagged)
-  end.
-
-Function compile2_flagged_aspect_specification_f (a: aspect_specification): aspect_specification_x :=
-  match a with
-  | mkaspect_specification ast_num mk e =>
-      let e_flagged := compile2_flagged_exp_f e in
-        (mkaspect_specification_x ast_num mk e_flagged)
-  end.
-
-Function compile2_flagged_aspect_specifications_f (la: list aspect_specification): list aspect_specification_x :=
-  match la with
-  | nil => nil
-  | a :: la' =>
-      let a_flagged := compile2_flagged_aspect_specification_f a in
-      let la_flagged := compile2_flagged_aspect_specifications_f la' in
-        (a_flagged :: la_flagged)
+        param_flagged :: lparam_flagged
   end.
 
 
-Function compile2_flagged_declaration_f (d: declaration): declaration_x :=
+Function compile2_flagged_declaration_f (st: symboltable) (d: declaration): option declaration_x :=
   match d with
-  | D_Null_Declaration => D_Null_Declaration_X
+  | D_Null_Declaration => Some D_Null_Declaration_X
   | D_Type_Declaration ast_num t =>
       let t_flagged := compile2_flagged_type_declaration_f t in
-        (D_Type_Declaration_X ast_num t_flagged)
+        Some (D_Type_Declaration_X ast_num t_flagged)
   | D_Object_Declaration ast_num o =>
       let o_flagged := compile2_flagged_object_declaration_f o in
-        (D_Object_Declaration_X ast_num o_flagged)
+        Some (D_Object_Declaration_X ast_num o_flagged)
   | D_Procedure_Body ast_num p =>
-      let p_flagged := compile2_flagged_procedure_body_f p in
-        (D_Procedure_Body_X ast_num p_flagged)
+      match compile2_flagged_procedure_body_f st p with
+      | Some p_flagged => Some (D_Procedure_Body_X ast_num p_flagged)
+      | None           => None
+      end
   | D_Seq_Declaration ast_num d1 d2 =>
-      let d1_flagged := compile2_flagged_declaration_f d1 in
-      let d2_flagged := compile2_flagged_declaration_f d2 in
-        (D_Seq_Declaration_X ast_num d1_flagged d2_flagged)
+      match compile2_flagged_declaration_f st d1 with
+      | Some d1_flagged =>
+          match compile2_flagged_declaration_f st d2 with
+          | Some d2_flagged => Some (D_Seq_Declaration_X ast_num d1_flagged d2_flagged)
+          | None            => None
+          end
+      | None            => None
+      end
   end
 
-with compile2_flagged_procedure_body_f (p: procedure_body): procedure_body_x :=
+with compile2_flagged_procedure_body_f (st: symboltable) (p: procedure_body): option procedure_body_x :=
   match p with
-  | mkprocedure_body ast_num p params aspects decls stmt =>
-      let aspects_flagged := compile2_flagged_aspect_specifications_f aspects in
+  | mkprocedure_body ast_num p params decls stmt =>
       let params_flagged := compile2_flagged_parameter_specifications_f params in
-      let decls_flagged := compile2_flagged_declaration_f decls in
-      let stmt_flagged := compile2_flagged_stmt_f stmt in
-        (mkprocedure_body_x ast_num p params_flagged aspects_flagged decls_flagged stmt_flagged)
+        match compile2_flagged_declaration_f st decls with
+        | Some decls_flagged =>
+          match compile2_flagged_stmt_f st stmt with
+          | Some stmt_flagged => Some (mkprocedure_body_x ast_num p params_flagged decls_flagged stmt_flagged)
+          | None              => None
+          end
+        | None               => None
+        end
   end.
-
-(*
-Function compile2_flagged_declaration_f11 (d: declaration): declaration_x :=
-  match d with
-  | D_Null_Declaration => D_Null_Declaration_X
-  | D_Object_Declaration ast_num o =>
-      let o_flagged := compile2_flagged_object_declaration_f o in
-        (D_Object_Declaration_X ast_num o_flagged)
-  | D_Type_Declaration ast_num t =>
-      let t_flagged := compile2_flagged_type_declaration_f t in
-        (D_Type_Declaration_X ast_num t_flagged)
-  | D_Procedure_Body ast_num p =>
-      let p_flagged :=
-          match p with
-          | mkprocedure_body ast_num p params aspects decls stmt =>
-              let aspects_flagged := compile2_flagged_aspect_specifications_f aspects in
-              let params_flagged := compile2_flagged_parameter_specifications_f params in
-              let decls_flagged := compile2_flagged_declaration_f decls in
-              let stmt_flagged := compile2_flagged_stmt_f stmt in
-                (mkprocedure_body_x ast_num p params_flagged aspects_flagged decls_flagged stmt_flagged)
-          end in
-        (D_Procedure_Body_X ast_num p_flagged)
-  | D_Seq_Declaration ast_num d1 d2 =>
-      let d1_flagged := compile2_flagged_declaration_f d1 in
-      let d2_flagged := compile2_flagged_declaration_f d2 in
-        (D_Seq_Declaration_X ast_num d1_flagged d2_flagged)
-  end.
-*)
 
 
 (* ***************************************************************
@@ -366,62 +442,93 @@ Function compile2_flagged_declaration_f11 (d: declaration): declaration_x :=
 Scheme expression_ind := Induction for expression Sort Prop 
                          with name_ind := Induction for name Sort Prop.
 
-Lemma compile2_flagged_exp_f_correctness: forall e e',
-  compile2_flagged_exp_f e = e' ->
-    compile2_flagged_exp e e'.
+Lemma compile2_flagged_exp_f_correctness: forall e e' checkflags,
+  compile2_flagged_exp_f checkflags e = e' ->
+    compile2_flagged_exp checkflags e e'.
 Proof.
   apply (expression_ind
-    (fun e: expression => forall (e' : expression_x),
-      compile2_flagged_exp_f e = e' ->
-      compile2_flagged_exp e e')
-    (fun n: name => forall (n': name_x),
-      compile2_flagged_name_f n = n' ->
-      compile2_flagged_name n n')
+    (fun e: expression => forall (e' : expression_x) (checkflags: check_flags),
+      compile2_flagged_exp_f checkflags e = e' ->
+      compile2_flagged_exp checkflags e e')
+    (fun n: name => forall (n': name_x) (checkflags: check_flags),
+      compile2_flagged_name_f checkflags n = n' ->
+      compile2_flagged_name checkflags n n')
     ); smack;
-  [destruct l | | destruct b | destruct u | | | ];
-  repeat progress constructor; smack.
+  [ | | 
+    destruct b; constructor; smack | 
+    destruct u; constructor; smack | | | 
+  ];
+  constructor; apply H; auto.
 Qed.
 
-Lemma compile2_flagged_name_f_correctness: forall e e',
-  compile2_flagged_name_f e = e' ->
-    compile2_flagged_name e e'.
+Lemma compile2_flagged_name_f_correctness: forall n n' checkflags,
+  compile2_flagged_name_f checkflags n = n' ->
+    compile2_flagged_name checkflags n n'.
 Proof.
   intros.
-  destruct e; smack;
+  destruct n; smack;
   repeat progress constructor;
-  apply compile2_flagged_exp_f_correctness; auto.  
+  apply compile2_flagged_exp_f_correctness; auto.
 Qed.
 
-Lemma compile2_flagged_exps_f_correctness: forall le le',
-  compile2_flagged_exps_f le = le' ->
-    compile2_flagged_exps le le'.
+Lemma compile2_flagged_args_f_correctness: forall params args args',
+  compile2_flagged_args_f params args = Some args' ->
+    compile2_flagged_args params args args'.
 Proof.
-  induction le; smack.
-- constructor.
-- constructor.
-  + apply compile2_flagged_exp_f_correctness; auto.
-  + auto.
+  induction params; smack.
+- destruct args; smack.
+  constructor.
+- destruct args; smack.
+  remember (is_range_constrainted_type (parameter_subtype_mark a)) as x.
+  remember (compile2_flagged_args_f params args) as y.
+  destruct x, y; smack;
+  [ apply C2_Flagged_Args_R |
+    apply C2_Flagged_Args
+  ]; smack;
+  apply compile2_flagged_exp_f_correctness; auto.
 Qed.
   
-Lemma compile2_flagged_stmt_f_correctness: forall c c',
-  compile2_flagged_stmt_f c = c' ->
-    compile2_flagged_stmt c c'.
+Lemma compile2_flagged_stmt_f_correctness: forall st c c',
+  compile2_flagged_stmt_f st c = Some c' ->
+    compile2_flagged_stmt st c c'.
 Proof.
   induction c; smack.
 - constructor.
-- constructor;
-  [ apply compile2_flagged_name_f_correctness |
-    apply compile2_flagged_exp_f_correctness 
-  ]; auto.
-- constructor;
+- remember (fetch_exp_type (name_astnum n) st) as x;
+  destruct x; smack.
+  remember (is_range_constrainted_type t) as y.
+  destruct y; smack;
+  [apply C2_Flagged_Assignment_R with (t := t); smack |
+   apply C2_Flagged_Assignment with (t := t); smack 
+  ];
+  [apply compile2_flagged_name_f_correctness; auto | | 
+   apply compile2_flagged_name_f_correctness; auto | 
+  ];
+  apply compile2_flagged_exp_f_correctness; auto.
+- remember (compile2_flagged_stmt_f st c1) as x;
+  destruct x; smack.
+  remember (compile2_flagged_stmt_f st c2) as y;
+  destruct y; smack.
+  constructor;
   [ apply compile2_flagged_exp_f_correctness | | ];
   smack.
-- constructor;
+- remember (compile2_flagged_stmt_f st c) as x;
+  destruct x; smack.
+  constructor;
   [ apply compile2_flagged_exp_f_correctness | ];
   smack.
-- constructor;
-  apply compile2_flagged_exps_f_correctness; auto.
-- constructor; auto.
+- remember (fetch_proc p st) as x;
+  destruct x; smack.
+  destruct t.
+  remember (compile2_flagged_args_f (procedure_parameter_profile p0) l) as y;
+  destruct y; smack.
+  apply C2_Flagged_Procedure_Call with (n := l0) (pb := p0) (params := (procedure_parameter_profile p0)); smack.
+  apply compile2_flagged_args_f_correctness; auto.
+- remember (compile2_flagged_stmt_f st c1) as x;
+  destruct x; smack.
+  remember (compile2_flagged_stmt_f st c2) as y;
+  destruct y; smack.
+  constructor; auto.
 Qed.
 
 Lemma compile2_flagged_type_declaration_f_correctness: forall t t',
@@ -436,9 +543,12 @@ Lemma compile2_flagged_object_declaration_f_correctness: forall o o',
   compile2_flagged_object_declaration_f o = o' ->
     compile2_flagged_object_declaration o o'.
 Proof.
-  intros. 
+  intros;
   functional induction compile2_flagged_object_declaration_f o; smack;
-  constructor.
+  [constructor |
+   apply C2_Flagged_Object_Declaration_R; auto |
+   apply C2_Flagged_Object_Declaration; auto
+  ];
   apply compile2_flagged_exp_f_correctness; auto.
 Qed.
 
@@ -469,65 +579,54 @@ Proof.
   apply compile2_flagged_parameter_specification_f_correctness; auto.
 Qed.
 
-Lemma compile2_flagged_aspect_specification_f_correctness: forall a a',
-  compile2_flagged_aspect_specification_f a = a' ->
-    compile2_flagged_aspect_specification a a'.
-Proof.
-  smack;
-  destruct a; constructor.
-  apply compile2_flagged_exp_f_correctness; auto.
-Qed.
-
-Lemma compile2_flagged_aspect_specifications_f_correctness: forall la la',
-  compile2_flagged_aspect_specifications_f la = la' ->
-    compile2_flagged_aspect_specifications la la'.
-Proof.
-  induction la; smack;
-  constructor; smack.
-  apply compile2_flagged_aspect_specification_f_correctness; auto.
-Qed.
-
 
 Scheme declaration_ind := Induction for declaration Sort Prop 
                           with procedure_body_ind := Induction for procedure_body Sort Prop.
 
-Lemma compile2_flagged_declaration_f_correctness: forall d d',
-  compile2_flagged_declaration_f d = d' ->
-    compile2_flagged_declaration d d'.
+Lemma compile2_flagged_declaration_f_correctness: forall d d' st,
+  compile2_flagged_declaration_f st d = Some d' ->
+    compile2_flagged_declaration st d d'.
 Proof.
   apply (declaration_ind
-    (fun d: declaration => forall (d' : declaration_x),
-      compile2_flagged_declaration_f d = d' ->
-      compile2_flagged_declaration d d')
-    (fun p: procedure_body => forall (p': procedure_body_x),
-      compile2_flagged_procedure_body_f p = p' ->
-      compile2_flagged_procedure_body p p')
+    (fun d: declaration => forall (d' : declaration_x) (st: symboltable),
+      compile2_flagged_declaration_f st d = Some d' ->
+      compile2_flagged_declaration st d d')
+    (fun p: procedure_body => forall (p': procedure_body_x) (st: symboltable),
+      compile2_flagged_procedure_body_f st p = Some p' ->
+      compile2_flagged_procedure_body st p p')
     ); smack.
 - constructor.
 - constructor.
   apply compile2_flagged_type_declaration_f_correctness; auto.
 - constructor.
   apply compile2_flagged_object_declaration_f_correctness; auto.
-- constructor;
-  smack.
-- constructor;
-  smack.
-- constructor.
-  apply compile2_flagged_aspect_specifications_f_correctness; auto.
-  apply compile2_flagged_parameter_specifications_f_correctness; auto.
-  smack.
-  apply compile2_flagged_stmt_f_correctness; auto.
+- remember (compile2_flagged_procedure_body_f st p) as x; 
+  destruct x; smack.
+  constructor; auto.
+- remember (compile2_flagged_declaration_f st d) as x;
+  remember (compile2_flagged_declaration_f st d0) as y;
+  destruct x, y; smack.  
+  constructor; smack.
+- remember (compile2_flagged_declaration_f st procedure_declarative_part) as x;
+  remember (compile2_flagged_stmt_f st procedure_statements) as y;
+  destruct x, y; smack.
+  constructor;
+  [ apply compile2_flagged_parameter_specifications_f_correctness | |
+    apply compile2_flagged_stmt_f_correctness
+  ]; auto.
 Qed.
 
-Lemma compile2_flagged_procedure_declaration_f_correctness: forall p p',
-  compile2_flagged_procedure_body_f p = p' ->
-    compile2_flagged_procedure_body p p'.
+Lemma compile2_flagged_procedure_declaration_f_correctness: forall st p p',
+  compile2_flagged_procedure_body_f st p = Some p' ->
+    compile2_flagged_procedure_body st p p'.
 Proof.
   intros;
-  destruct p; smack;
+  destruct p; smack.
+  remember (compile2_flagged_declaration_f st procedure_declarative_part) as x;
+  remember (compile2_flagged_stmt_f st procedure_statements) as y;
+  destruct x, y; smack.  
   constructor;
-  [ apply compile2_flagged_aspect_specifications_f_correctness |
-    apply compile2_flagged_parameter_specifications_f_correctness |
+  [ apply compile2_flagged_parameter_specifications_f_correctness |
     apply compile2_flagged_declaration_f_correctness |
     apply compile2_flagged_stmt_f_correctness 
   ]; auto.
@@ -538,24 +637,78 @@ Qed.
 
 Require Import X_SparkTactics.
 
-Lemma procedure_components_rel: forall p p',
-  compile2_flagged_procedure_body p p' ->
+Lemma procedure_components_rel: forall st p p',
+  compile2_flagged_procedure_body st p p' ->
   compile2_flagged_parameter_specifications (procedure_parameter_profile p) (procedure_parameter_profile_x p') /\
-  compile2_flagged_declaration (procedure_declarative_part p) (procedure_declarative_part_x p') /\
-  compile2_flagged_stmt (procedure_statements p) (procedure_statements_x p').
+  compile2_flagged_declaration st (procedure_declarative_part p) (procedure_declarative_part_x p') /\
+  compile2_flagged_stmt st (procedure_statements p) (procedure_statements_x p').
 Proof.
   intros.
   inversion H; smack.
 Qed.
 
 
+(** * Compile To Flagged Symbol Table *)
 
 
+Inductive compile2_flagged_proc_declaration_map: symboltable ->
+                                                 list (idnum * (level * procedure_body)) -> 
+                                                 list (idnum * (level * procedure_body_x)) -> Prop :=
+    | C2_Flagged_Proc_Declaration_Map_Null: forall st,
+        compile2_flagged_proc_declaration_map st nil nil
+    | C2_Flagged_Proc_Declaration_Map: forall st pb pb' pl pl' p l,
+        compile2_flagged_procedure_body st pb pb' ->
+        compile2_flagged_proc_declaration_map st pl pl' ->
+        compile2_flagged_proc_declaration_map st ((p, (l, pb)) :: pl) ((p, (l, pb')) :: pl').
+
+Inductive compile2_flagged_type_declaration_map: list (idnum * type_declaration) -> 
+                                                 list (idnum * type_declaration_x) -> Prop :=
+    | C2_Flagged_Type_Declaration_Map_Null:
+        compile2_flagged_type_declaration_map nil nil
+    | C2_Flagged_Type_Declaration_Map: forall t t' tl tl' x,
+        compile2_flagged_type_declaration t t' ->
+        compile2_flagged_type_declaration_map tl tl' ->
+        compile2_flagged_type_declaration_map ((x, t) :: tl) ((x, t') :: tl').
+
+Inductive compile2_flagged_symbol_table: symboltable -> symboltable_x -> Prop := 
+  | C2_Flagged_SymTable: forall p p' t t' x e,
+      compile2_flagged_proc_declaration_map (mkSymbolTable x p t e) p p' ->
+      compile2_flagged_type_declaration_map t t' ->
+      compile2_flagged_symbol_table (mkSymbolTable x p t e) (mkSymbolTable_x x p' t' e).
 
 
+(** ** Lemmas *)
 
+Lemma procedure_declaration_rel: forall st ps ps' p n pb n' pb',
+  compile2_flagged_proc_declaration_map st ps ps' ->
+    Symbol_Table_Module.SymTable_Procs.fetches p ps = Some (n, pb) ->
+      Symbol_Table_Module_X.SymTable_Procs.fetches p ps' = Some (n', pb') ->
+        n = n' /\ compile2_flagged_procedure_body st pb pb'.
+Proof.
+  intros st ps ps' p n pb n' pb' H; revert p n pb n' pb'.
+  induction H; intros.
+- inversion H; inversion H0; auto.
+- unfold Symbol_Table_Module.SymTable_Procs.fetches in H1;
+  unfold Symbol_Table_Module_X.SymTable_Procs.fetches in H2.
+  remember (beq_nat p0 p) as Beq.
+  destruct Beq. 
+  + smack.
+  + specialize (IHcompile2_flagged_proc_declaration_map _ _ _ _ _ H1 H2).
+    auto.
+Qed.
 
-
-
-
+Lemma symbol_table_procedure_rel: forall p st n pb st' n' pb',
+  Symbol_Table_Module.fetch_proc p st = Some (n, pb) ->
+    Symbol_Table_Module_X.fetch_proc p st' = Some (n', pb') ->
+      compile2_flagged_symbol_table st st' ->
+        n = n' /\ compile2_flagged_procedure_body st pb pb'.
+Proof.
+  intros.
+  inversion H1; subst; clear H1.
+  unfold Symbol_Table_Module_X.fetch_proc in H0;
+  unfold Symbol_Table_Module.fetch_proc in H;
+  simpl in H0, H.
+  specialize (procedure_declaration_rel _ _ _ _ _ _ _ _ H2 H H0);
+  auto.
+Qed.
 
