language_formal/spark2014_semantics/spark2014_core_subset(non-nested)/symboltable.v
@@ -1,5 +1,5 @@
 Require Export symboltable_module.
-Require Export checks_generator.
+Require Export language_flagged.
 
 (** * Symbol Tables *)
 
@@ -9,91 +9,51 @@ Module Symbol_Table_Elements <: SymTable_Element.
   Definition Type_Decl := type_declaration.
 End Symbol_Table_Elements.
 
-Module Symbol_Table_Module := SymbolTableM (Symbol_Table_Elements).
-
-
 (* symbol table for flagged program *)
 Module Symbol_Table_Elements_X <: SymTable_Element.
   Definition Procedure_Decl := procedure_body_x.
   Definition Type_Decl := type_declaration_x.
 End Symbol_Table_Elements_X.
 
+Module Symbol_Table_Module := SymbolTableM (Symbol_Table_Elements).
+
 Module Symbol_Table_Module_X := SymbolTableM (Symbol_Table_Elements_X).
 
-
-
-(** * Compile To Flagged Symbol Table *)
-
-Definition symbol_table := Symbol_Table_Module.symboltable.
-Definition symbol_table' := Symbol_Table_Module_X.symboltable.
-
+Definition symboltable := Symbol_Table_Module.symboltable.
 Definition mkSymbolTable := Symbol_Table_Module.mkSymbolTable.
-Definition mkSymbolTable' := Symbol_Table_Module_X.mkSymbolTable.
-
 Definition proc_decl := Symbol_Table_Module.proc_decl.
 Definition type_decl := Symbol_Table_Module.type_decl.
-Definition proc_decl' := Symbol_Table_Module_X.proc_decl.
-Definition type_decl' := Symbol_Table_Module_X.type_decl.
+
+Definition symboltable_x := Symbol_Table_Module_X.symboltable.
+Definition mkSymbolTable_x := Symbol_Table_Module_X.mkSymbolTable.
+Definition proc_decl_x := Symbol_Table_Module_X.proc_decl.
+Definition type_decl_x := Symbol_Table_Module_X.type_decl.
 
 Definition level := Symbol_Table_Module.level.
 
-Inductive compile2_flagged_proc_declaration_map: list (idnum * (level * procedure_body)) -> 
-                                                 list (idnum * (level * procedure_body_x)) -> Prop :=
-    | C2_Flagged_Proc_Declaration_Map_Null:
-        compile2_flagged_proc_declaration_map nil nil
-    | C2_Flagged_Proc_Declaration_Map: forall pd pd' pl pl' p l,
-        compile2_flagged_procedure_body pd pd' ->
-        compile2_flagged_proc_declaration_map pl pl' ->
-        compile2_flagged_proc_declaration_map ((p, (l, pd)) :: pl) ((p, (l, pd')) :: pl').
+Definition reside_symtable_vars := Symbol_Table_Module.reside_symtable_vars.
+Definition reside_symtable_procs := Symbol_Table_Module.reside_symtable_procs.
+Definition reside_symtable_types := Symbol_Table_Module.reside_symtable_types.
+Definition reside_symtable_exps := Symbol_Table_Module.reside_symtable_exps.
+Definition fetch_var := Symbol_Table_Module.fetch_var.
+Definition fetch_proc := Symbol_Table_Module.fetch_proc.
+Definition fetch_type := Symbol_Table_Module.fetch_type.
+Definition fetch_exp_type := Symbol_Table_Module.fetch_exp_type.
+Definition update_vars := Symbol_Table_Module.update_vars.
+Definition update_procs := Symbol_Table_Module.update_procs.
+Definition update_types := Symbol_Table_Module.update_types.
+Definition update_exps := Symbol_Table_Module.update_exps.
 
-Inductive compile2_flagged_type_declaration_map: list (idnum * type_declaration) -> 
-                                                 list (idnum * type_declaration_x) -> Prop :=
-    | C2_Flagged_Type_Declaration_Map_Null:
-        compile2_flagged_type_declaration_map nil nil
-    | C2_Flagged_Type_Declaration_Map: forall t t' tl tl' x,
-        compile2_flagged_type_declaration t t' ->
-        compile2_flagged_type_declaration_map tl tl' ->
-        compile2_flagged_type_declaration_map ((x, t) :: tl) ((x, t') :: tl').
-
-Inductive compile2_flagged_symbol_table: symbol_table -> symbol_table' -> Prop := 
-  | C2_Flagged_SymTable: forall p p' t t' x,
-      compile2_flagged_proc_declaration_map p p' ->
-      compile2_flagged_type_declaration_map t t' ->
-      compile2_flagged_symbol_table (mkSymbolTable x p t) (mkSymbolTable' x p' t').
-
-
-(** * Lemmas *)
-
-Lemma procedure_declaration_rel: forall ps ps' p n pb n' pb',
-  compile2_flagged_proc_declaration_map ps ps' ->
-    Symbol_Table_Module.SymTable_Procs.fetches p ps = Some (n, pb) ->
-      Symbol_Table_Module_X.SymTable_Procs.fetches p ps' = Some (n', pb') ->
-        n = n' /\ compile2_flagged_procedure_body pb pb'.
-Proof.
-  intros ps ps' p n pb n' pb' H; revert p n pb n' pb'.
-  induction H; intros.
-- inversion H; inversion H0; auto.
-- unfold Symbol_Table_Module.SymTable_Procs.fetches in H1;
-  unfold Symbol_Table_Module_X.SymTable_Procs.fetches in H2.
-  remember (beq_nat p0 p) as Beq.
-  destruct Beq. 
-  + smack.
-  + specialize (IHcompile2_flagged_proc_declaration_map _ _ _ _ _ H1 H2).
-    auto.
-Qed.
-
-Lemma symbol_table_procedure_rel: forall p st n pb st' n' pb',
-  Symbol_Table_Module.fetch_proc p st = Some (n, pb) ->
-    Symbol_Table_Module_X.fetch_proc p st' = Some (n', pb') ->
-      compile2_flagged_symbol_table st st' ->
-        n = n' /\ compile2_flagged_procedure_body pb pb'.
-Proof.
-  intros.
-  inversion H1; subst; clear H1.
-  unfold Symbol_Table_Module_X.fetch_proc in H0;
-  unfold Symbol_Table_Module.fetch_proc in H;
-  simpl in H0, H.
-  specialize (procedure_declaration_rel _ _ _ _ _ _ _ H2 H H0);
-  auto.
-Qed.
+Definition reside_symtable_vars_x := Symbol_Table_Module_X.reside_symtable_vars.
+Definition reside_symtable_procs_x := Symbol_Table_Module_X.reside_symtable_procs.
+Definition reside_symtable_types_x := Symbol_Table_Module_X.reside_symtable_types.
+Definition reside_symtable_exps_x := Symbol_Table_Module_X.reside_symtable_exps.
+Definition fetch_var_x := Symbol_Table_Module_X.fetch_var.
+Definition fetch_proc_x := Symbol_Table_Module_X.fetch_proc.
+Definition fetch_type_x := Symbol_Table_Module_X.fetch_type.
+Definition fetch_exp_type_x := Symbol_Table_Module_X.fetch_exp_type.
+Definition update_vars_x := Symbol_Table_Module_X.update_vars.
+Definition update_procs_x := Symbol_Table_Module_X.update_procs.
+Definition update_types_x := Symbol_Table_Module_X.update_types.
+Definition update_exps_x := Symbol_Table_Module_X.update_exps.
 
